WBAssn proofs

Lean/Geo/NGon/WBAssnNew.lean
@@ -15,11 +15,11 @@ open Point
 
 def isCap (w : WBPoints) (a c d : Fin w.length) (o : Orientation) :=
   ∃ b, a < b ∧ b < c ∧ c < d ∧
-    σ w[a] w[b] w[c] = o ∧ σ w[a] w[c] w[d] = o
+    σ w[a] w[b] w[c] = o ∧ σ w[b] w[c] w[d] = o
 
-def isCapF (w : WBPoints) (a d e : Fin w.length) :=
-  ∃ c : Fin w.length, isCap w a c d .CW ∧
-    σ w[c] w[d] w[e] = .CW ∧ σIsEmptyTriangleFor w[a] w[c] w[e] w.toFinset
+def isCapF (w : WBPoints) (a c d : Fin w.length) :=
+  c < d ∧ ∃ b : Fin w.length, isCap w a b c .CW ∧
+    σ w[b] w[c] w[d] = .CW ∧ σIsEmptyTriangleFor w[a] w[b] w[d] w.toFinset
 
 @[simp] def toPropAssn (w : WBPoints) : Var w.length → Prop
   | .sigma a b c    => σ w[a] w[b] w[c] = .CCW
@@ -31,19 +31,12 @@ def isCapF (w : WBPoints) (a d e : Fin w.length) :=
 
 attribute [-simp] getElem_fin
 
-theorem satisfies_signotopeClauses (w : WBPoints) : (signotopeClauses w.length).eval w.toPropAssn := by
+theorem satisfies_signotopeClauses (w : WBPoints) :
+    (signotopeClauses w.length).eval w.toPropAssn := by
   simp [signotopeClauses]
   intro i j hij k hjk l hkl
-  have : [w[i], w[j], w[k], w[l]] <+ w.points := by
-    have : [w[i], w[j], w[k], w[l]] = [i,j,k,l].map w.points.get := by
-      simp [GetElem.getElem, List.getElem_eq_get]
-    rw [this]
-    apply map_get_sublist
-    have := hjk.trans hkl
-    simp [hij, hjk, hkl, hij.trans hjk, hij.trans this, this]
-  have s : Sorted₄ w[i] w[j] w[k] w[l] := w.sorted.to₄ this
-  have gp : InGeneralPosition₄ w[i] w[j] w[k] w[l] :=
-    PointListInGeneralPosition.to₄ w.gp this
+  have s : Sorted₄ w[i] w[j] w[k] w[l] := w.sorted₄ hij hjk hkl
+  have gp : InGeneralPosition₄ w[i] w[j] w[k] w[l] := w.gp₄ hij hjk hkl
   constructor
   . exact σ_prop₂ s gp
   constructor
@@ -84,7 +77,8 @@ theorem insideDefs_aux₂ {a b x c : Point} : Sorted₄ a b x c → InGeneralPos
     σ_perm₂ b c x,
     σ_perm₂ b c a, σ_perm₁ b a c,
     gp.gp₄.σ_iff]
-  cases gp.gp₁.σ_cases <;> cases gp.gp₂.σ_cases <;> cases gp.gp₃.σ_cases <;> cases gp.gp₄.σ_cases <;> simp_all
+  cases gp.gp₁.σ_cases <;> cases gp.gp₂.σ_cases <;>
+    cases gp.gp₃.σ_cases <;> cases gp.gp₄.σ_cases <;> simp_all
   next h₁ h₂ h₃ h₄ =>
     rw [σ_prop₁ sorted gp h₁ h₄] at h₃
     contradiction
@@ -97,49 +91,28 @@ theorem satisfies_insideClauses (w : WBPoints) : (insideClauses w.length).eval w
   intro a b hab c hbc x
   constructor
   · intro hax hxb
-    have : [w[a], w[x], w[b], w[c]] <+ w.points := by
-      have : [w[a], w[x], w[b], w[c]] = [a,x,b,c].map w.points.get := by
-        simp [GetElem.getElem, List.getElem_eq_get]
-      rw [this]
-      apply map_get_sublist
-      have : a < c := hab.trans hbc
-      have : x < c := hxb.trans hbc
-      simp [*]
-    exact (insideDefs_aux₁ (w.sorted.to₄ this) (PointListInGeneralPosition.to₄ w.gp this)).1
+    exact (insideDefs_aux₁ (w.sorted₄ hax hxb hbc) (w.gp₄ hax hxb hbc)).1
   · intro hbx hxc
-    have : [w[a], w[b], w[x], w[c]] <+ w.points := by
-      have : [w[a], w[b], w[x], w[c]] = [a,b,x,c].map w.points.get := by
-        simp [GetElem.getElem, List.getElem_eq_get]
-      rw [this]
-      apply map_get_sublist
-      have : a < x := hab.trans hbx
-      have : a < c := hab.trans hbc
-      simp [*]
-    exact (insideDefs_aux₂ (w.sorted.to₄ this) (PointListInGeneralPosition.to₄ w.gp this)).1
+    exact (insideDefs_aux₂ (w.sorted₄ hab hbx hxc) (w.gp₄ hab hbx hxc)).1
 
 theorem satisfies_holeDefClauses (w : WBPoints) : (holeDefClauses w.length).eval w.toPropAssn := by
   simp [holeDefClauses, σIsEmptyTriangleFor, mem_toFinset_iff]
   intro a b ab c bc H i tri
-  have sub : [w[a],w[b],w[c]] <+ w.points := by
-    have : [w[a],w[b],w[c]] = [a,b,c].map w.points.get := by
-      simp [GetElem.getElem, List.getElem_eq_get]
-    rw [this]
-    apply map_get_sublist
-    aesop (add unsafe lt_trans)
-  have gp₄ : InGeneralPosition₄ w[i] w[a] w[b] w[c] := tri.gp₄_of_gp₃ (w.gp sub)
+  have gp₄ : InGeneralPosition₄ w[i] w[a] w[b] w[c] := tri.gp₄_of_gp₃ (w.gp₃ ab bc)
   have ib : i ≠ b := mt (congrArg (w[·])) gp₄.gp₃.ne₁
-  have ⟨wawi, wiwc⟩ := xBounded_of_PtInTriangle' (w.sorted.to₃ sub) ((σPtInTriangle_iff gp₄).mp tri)
-  have ai : a < i := w.of_sorted_get <| by
+  have ⟨wawi, wiwc⟩ := xBounded_of_PtInTriangle' (w.sorted₃ ab bc) ((σPtInTriangle_iff gp₄).mp tri)
+  have ai : a < i := w.lt_iff.1 <| by
     apply lt_of_le_of_ne wawi
     intro h
-    exact gp₄.gp₁.ne₁ <| w.of_eqx h.symm ▸ rfl
-  have ic : i < c := w.of_sorted_get <| by
+    exact gp₄.gp₁.ne₁ <| w.eq_iff.1 h.symm ▸ rfl
+  have ic : i < c := w.lt_iff.1 <| by
     apply lt_of_le_of_ne wiwc
     intro h
-    exact gp₄.gp₃.ne₂ <| w.of_eqx h ▸ rfl
+    exact gp₄.gp₃.ne₂ <| w.eq_iff.1 h ▸ rfl
   exact H i ai ic ib tri
 
-theorem satisfies_leftmostCCWDefs (w : WBPoints) : (leftmostCCWClauses w.length).eval w.toPropAssn := by
+theorem satisfies_leftmostCCWDefs (w : WBPoints) :
+    (leftmostCCWClauses w.length).eval w.toPropAssn := by
   simp [leftmostCCWClauses]
   intro i h0i j hij
   let ⟨i+1, hi⟩ := i; let ⟨j+1, hj⟩ := j
@@ -177,8 +150,84 @@ theorem satisfies_triangleEncoding (w : WBPoints) :
   simp [triangleEncoding, satisfies_baseEncoding, noHoleClauses,
     σIsEmptyTriangleFor, mem_toFinset_iff, σHasEmptyTriangle]
   intro noholes a b hab c hbc
-  exact noholes a b (ne_of_lt hab <| w.of_eqx <| · ▸ rfl)
-                  c (ne_of_lt (hab.trans hbc) <| w.of_eqx <| · ▸ rfl)
-                    (ne_of_lt hbc <| w.of_eqx <| · ▸ rfl)
+  exact noholes a b (ne_of_lt hab <| w.eq_iff.1 <| · ▸ rfl)
+                  c (ne_of_lt (hab.trans hbc) <| w.eq_iff.1 <| · ▸ rfl)
+                    (ne_of_lt hbc <| w.eq_iff.1 <| · ▸ rfl)
+
+theorem satisfies_capDef (w : WBPoints) {a b c d : Fin (length w)}
+    (ab : a < b) (bc : b < c) (cd : c < d) : (capDef a b c d).eval w.toPropAssn := by
+  simp [capDef, isCap]; intro h1 h2
+  exact ⟨_, ab, bc, cd, (w.gp₃ ab bc).σ_iff.1 h1, (w.gp₃ bc cd).σ_iff.1 h2⟩
+
+theorem satisfies_capDef2 (w : WBPoints) {a c d : Fin (length w)} :
+    (capDef2 a c d).eval w.toPropAssn := by
+  simp [capDef2, isCap]; intro b ab bc cd h1 h2
+  have gp := w.gp₄ ab bc cd
+  exact gp.gp₃.σ_iff.2 <| σ_prop₃ (w.sorted₄ ab bc cd) gp h1 h2
+
+theorem satisfies_cupDef (w : WBPoints) {a b c d : Fin (length w)}
+    (ab : a < b) (bc : b < c) (cd : c < d) : (cupDef a b c d).eval w.toPropAssn := by
+  simp [cupDef, isCap]; intro h1 h2
+  exact ⟨_, ab, bc, cd, h1, h2⟩
+
+theorem satisfies_cupDef2 (w : WBPoints) {a c d : Fin (length w)} :
+    (cupDef2 a c d).eval w.toPropAssn := by
+  simp [cupDef2, isCap]; intro b ab bc cd h1 h2
+  exact σ_prop₁ (w.sorted₄ ab bc cd) (w.gp₄ ab bc cd) h1 h2
+
+theorem satisfies_capFDef (w : WBPoints) {a b c d : Fin (length w)} (bc : b < c) (cd : c < d)
+    (hh : σIsEmptyTriangleFor w[a] w[b] w[d] w.toFinset) : (capFDef a b c d).eval w.toPropAssn := by
+  simp [capFDef, isCapF]; intro h1 h2
+  exact ⟨cd, _, h2, (w.gp₃ bc cd).σ_iff.1 h1, hh⟩
+
+theorem satisfies_no6Hole3Below {w : WBPoints} (hw : ¬σHasEmptyNGon 6 w.toFinset)
+    {a c d e : Fin (length w)}
+    (ha : (0 : Fin (w.rest.length+1)) < a) (de : d < e)
+    (ace : σIsEmptyTriangleFor w[a] w[c] w[e] w.toFinset) :
+    (no6Hole3Below a c d e).eval w.toPropAssn := by
+  simp [no6Hole3Below]; intro ⟨b, ab, bc, cd, abc, bcd⟩ cde
+  sorry
+
+theorem satisfies_no6Hole4Above {w : WBPoints} (hw : ¬σHasEmptyNGon 6 w.toFinset)
+    {a d e f : Fin (length w)}
+    (ha : (0 : Fin (w.rest.length+1)) < a) (ef : e < f) :
+    (no6Hole4Above a d e f).eval w.toPropAssn := by
+  simp [no6Hole4Above]; intro ⟨de, c, ⟨b, ab, bc, cd, abc, bcd⟩, cde, ace⟩
+  refine (w.gp₃ de ef).σ_iff'.1 fun def_ => ?_
+  sorry
+
+theorem satisfies_no6Hole2Below {w : WBPoints} (hw : ¬σHasEmptyNGon 6 w.toFinset)
+    {a c e f : Fin (length w)}
+    (ha : (0 : Fin (w.rest.length+1)) < a) (ce : c ≠ e) :
+    (no6Hole2Below a c f e).eval w.toPropAssn := by
+  simp [no6Hole2Below]; intro ⟨b, ab, bc, cf, abc, bcd⟩ ⟨d, ad, de, ef, ade, def_⟩ hh
+  split_ifs at hh with ce <;> simp at hh
+  · sorry
+  · replace ce := lt_of_le_of_ne (not_lt.1 ce) (Ne.symm ‹_›)
+    sorry
+
+theorem satisfies_no6Hole1Below {w : WBPoints} (hw : ¬σHasEmptyNGon 6 w.toFinset)
+    {a d e f : Fin (length w)}
+    (ha : (0 : Fin (w.rest.length+1)) < a) (df : d < f) (ae : a < e) (ef : e < f) (de : d ≠ e) :
+    (no6Hole1Below a d f e).eval w.toPropAssn := by
+  simp [no6Hole1Below]; intro ⟨df, c, ⟨b, ab, bc, cd, abc, bcd⟩, cdf, acf⟩ aef
+  sorry
+
+theorem satisfies_hexagonEncoding (w : WBPoints) (hw : ¬σHasEmptyNGon 6 w.toFinset) :
+    (hexagonEncoding w.length).eval w.toPropAssn := by
+  simp [hexagonEncoding, satisfies_baseEncoding, no6HoleClauses1, no6HoleClauses2, no6HoleClauses3]
+  refine ⟨
+    fun a ha b ab c bc d cd => ⟨?_, ?_, fun _ => ⟨fun hh => ⟨?_, ?_⟩, fun _ => ?_⟩⟩,
+    fun a _ b _ c _ => ⟨?_, ?_⟩,
+    fun a ha b _ c bc p ap pc bp => ⟨fun _ _ => ?_, fun _ => ?_⟩⟩
+  · with_reducible exact satisfies_capDef w ab bc cd
+  · with_reducible exact satisfies_cupDef w ab bc cd
+  · with_reducible exact satisfies_capFDef w bc cd hh
+  · with_reducible exact satisfies_no6Hole3Below hw ha cd hh
+  · with_reducible exact satisfies_no6Hole4Above hw ha cd
+  · with_reducible exact satisfies_capDef2 w
+  · with_reducible exact satisfies_cupDef2 w
+  · with_reducible exact satisfies_no6Hole2Below hw ha bp
+  · with_reducible exact satisfies_no6Hole1Below hw ha bc ap pc bp
 
 end WBPoints
